PROG_spec

theories/LambdaCalculus/Reductions/KrivineM_HALT_to_MMA_HALTING.v
@@ -8,12 +8,13 @@ Require Import PeanoNat List Lia.
 Import ListNotations.
 Require Import ssreflect ssrbool ssrfun.
 
-#[local] Notation mm_instr := (mm_instr (pos 6)).
-#[local] Notation counter := (pos 6).
-#[local] Notation mm_state := (mm_state 6).
+#[local] Notation mm_instr := (mm_instr (pos 5)).
+#[local] Notation counter := (pos 5).
+#[local] Notation mm_state := (mm_state 5).
 
 #[local] Notation "P // s -[ k ]-> t" := (sss_steps (@mma_sss _) P k s t).
 #[local] Notation "P // s ->> t" := (sss_compute (@mma_sss _) P s t).
+#[local] Notation "P // s -+> t" := (sss_progress (@mma_sss _) P s t).
 #[local] Notation "e #> x" := (vec_pos e x).
 #[local] Notation "e [ v / x ]" := (vec_change e x v).
 
@@ -39,23 +40,24 @@ Proof. move=> <-. by apply: vec_change_same. Qed.
 (* auxiliary counters *)
 Notation A := (Fin.F1 : counter).
 Notation B := (Fin.FS (Fin.F1) : counter).
-Notation C := (Fin.FS (Fin.FS (Fin.F1)) : counter).
 (* data counters *)
-Notation TS := (Fin.FS (Fin.FS (Fin.FS (Fin.F1))) : counter).
-Notation CTX := (Fin.FS (Fin.FS (Fin.FS (Fin.FS (Fin.F1)))) : counter).
-Notation U := (Fin.FS (Fin.FS (Fin.FS (Fin.FS (Fin.FS (Fin.F1))))) : counter).
+Notation TS := (Fin.FS (Fin.FS (Fin.F1)) : counter).
+Notation CTX := (Fin.FS (Fin.FS (Fin.FS (Fin.F1))) : counter).
+Notation U := (Fin.FS (Fin.FS (Fin.FS (Fin.FS (Fin.F1)))) : counter).
 
 (* simplify vec_change statements *)
 Definition vec_norm {X Y: counter} (HXY : X <> Y) := (
   fun v n m => @vec_change_comm nat _ v X Y n m HXY,
   fun v n m => @vec_change_idem nat _ v X n m,
   fun v n m => @vec_change_idem nat _ v Y n m,
-  fun v n => @vec_change_neq nat _  v X Y n HXY,
-  fun v n => @vec_change_neq nat _  v Y X n (nesym HXY),
-  fun v n => @vec_change_eq nat _  v X X n erefl,
-  fun v n => @vec_change_eq nat _  v Y Y n erefl).
+  fun v n => @vec_change_neq nat _ v X Y n HXY,
+  fun v n => @vec_change_neq nat _ v Y X n (nesym HXY),
+  fun v n => @vec_change_eq nat _ v X X n erefl,
+  fun v n => @vec_change_eq nat _ v Y Y n erefl,
+  fun v => @vec_change_same nat _ v X,
+  fun v => @vec_change_same nat _ v Y).
 
-Definition Q_step (Q : list mm_instr) (offset i : nat) (v : vec nat 6) : option mm_state :=
+Definition Q_step (Q : list mm_instr) (offset i : nat) (v : vec nat 5) : option mm_state :=
   match nth_error Q i with
   | None => None
   | Some (INC x) => Some ((S i) + offset, vec_change v x (S (vec_pos v x)))
@@ -68,7 +70,7 @@ Definition Q_step (Q : list mm_instr) (offset i : nat) (v : vec nat 6) : option 
 
 Lemma Q_step_spec (Q : list mm_instr) offset i v j w : 
   Q_step Q offset i v = Some (j, w) ->
-  sss_step (mma_sss (n:=6)) (offset, Q) (i + offset, v) (j, w).
+  sss_step (mma_sss (n:=5)) (offset, Q) (i + offset, v) (j, w).
 Proof.
   rewrite /Q_step. case E: (nth_error Q i) => [t|]; last done.
   move: E => /(@nth_error_split mm_instr) => - [l] [r] [-> <-].
@@ -144,20 +146,13 @@ Definition MOVE (X Y: counter) (offset: nat) : list mm_instr :=
 
 Definition MOVE_length := JMP_length+2.
 
-Lemma asd (P : counter -> Prop) : 
-  P A -> P B -> P C -> P TS -> P CTX -> P U -> forall (X : counter), P X.
+Lemma ext_counter (P : counter -> Prop) : 
+  P A -> P B -> P TS -> P CTX -> P U -> forall (X : counter), P X.
 Proof.
-Admitted.
-
-(* TODO use universaly 
-Definition simpl_vec_change {X Y : counter} (HXY : X <> Y) :=
-  (fun v n => @vec_change_neq nat _  v X Y n HXY,
-   fun v n => @vec_change_neq nat _  v Y X n (nesym HXY),
-   fun v n => @vec_change_eq nat _  v X X n erefl,
-   fun v n => @vec_change_eq nat _  v Y Y n erefl).
-*)
-
-
+  move=> ?????.
+  do 5 (move=> {}X; apply (Fin.caseS' X); first done).
+  by apply: Fin.case0.
+Qed.
 
 Lemma MOVE_spec X Y v offset :
   let x := vec_pos v X in
@@ -185,6 +180,55 @@ Proof.
     + by rewrite (vec_change_neq (nesym HXY)) vec_change_eq.
     + rewrite !(vec_norm HXY). congr vec_change. congr vec_change. lia.
 Qed.
+
+(* Y := X *)
+Definition COPY (X Y: counter) (offset: nat) : list mm_instr :=
+  let i := offset in JMP (2+JMP_length+i) i ++
+  let j := JMP_length + i in [INC A; INC Y] ++
+  let i := 2 + j in [DEC X j] ++
+  let i := 1 + i in MOVE A X i ++ [].
+
+Definition COPY_length := length (COPY A A 0).
+
+(* induction principle wrt. a decreasing measure f *)
+(* example: elim /(measure_ind length) : l. *)
+Lemma measure_ind {X : Type} (f : X -> nat) (P : X -> Prop) :
+  (forall x, (forall y, f y < f x -> P y) -> P x) -> forall (x : X), P x.
+Proof.
+  exact: (well_founded_ind (Wf_nat.well_founded_lt_compat X f _ (fun _ _ => id)) P).
+Qed.
+
+Lemma COPY_spec X Y v offset :
+  let x := vec_pos v X in let y := vec_pos v Y in let a := vec_pos v A in
+  A <> X -> A <> Y -> X <> Y ->
+  (offset, COPY X Y offset) // (offset, v) ->>
+    (COPY_length+offset, vec_change (vec_change (vec_change v X (a+x)) Y (x+y)) A 0).
+Proof.
+  move=> /= HX HY HXY. have H' : forall i, offset + i = i + offset by lia.
+  apply: sss_compute_trans.
+  { apply: (subcode_sss_compute (P := (_, JMP _ _))).
+    { by eexists [], _. }
+    rewrite ?H'. by apply: JMP_spec. }
+  move Ew: (vec_change _ A _) => w.
+  elim /(measure_ind (fun v => vec_pos v X)): v w Ew.
+  move=> v IH w <-. case Ex: (vec_pos v X) => [|x].
+  { apply: Q_step_spec'. { by rewrite /= Ex. }
+    apply: sss_compute_trans.
+    { apply: (subcode_sss_compute (P := (_, MOVE _ _ _))).
+      { eexists _, _. rewrite /COPY. by do 2 rewrite [LHS]app_assoc. }
+      rewrite ?H'. by apply: MOVE_spec. }
+    apply: sss_compute_refl'. congr pair.
+    congr vec_change. rewrite !(vec_norm HXY). congr vec_change. lia. }
+  apply: Q_step_spec'. { by rewrite /= Ex. }
+  apply: Q_step_spec'. { done. }
+  apply: Q_step_spec'. { done. }
+  apply: IH.
+  - rewrite !(vec_norm HXY) !(vec_norm HX). lia.
+  - do ? rewrite ?(vec_norm HX) ?(vec_norm HY) ?(vec_norm HXY).
+    congr vec_change. congr vec_change; last by lia.
+    congr vec_change. lia.
+Qed.
+
 
 (* X := X+X *)
 Definition DOUBLE (X: counter) (offset: nat) : list mm_instr :=
@@ -263,8 +307,6 @@ Proof.
     by move=> + _ H => /H.
 Qed.
 
-
-
 Lemma PACK_spec X Y v offset :
   let x := vec_pos v X in
   let y := vec_pos v Y in
@@ -327,23 +369,23 @@ Definition HALF (X: counter) (p q: nat) (offset: nat) : list mm_instr :=
 
 Definition HALF_length := length (HALF A 0 0 0).
 
-Fixpoint half (n: nat) : nat + nat :=
+(* second component is true iff n is even *)
+Fixpoint half (n: nat) : (nat * bool) :=
   match n with
-  | 0 => inl 0
+  | 0 => (0, true)
   | S n' => 
       match half n' with
-      | inl m => inr m
-      | inr m => inl (S m)
+      | (m, b) => if b then (m, false) else (S m, true)
       end
   end.
 
-Lemma half_spec n : 
+Lemma half_spec n :
   match half n with
-  | inl m => n = m + m
-  | inr m => n = 1 + m + m
+  | (m, b) => n = (if b then 0 else 1) + m + m
   end.
-Proof. elim: n => [|n] /=; [done|case: (half n); lia]. Qed.
+Proof. elim: n => [|n] /=; [done|case: (half n) => ? []; lia]. Qed.
 
+(*
 Lemma sig_half (n: nat) : { m | n = m + m } + { m | n = 1 + m + m }.
 Proof.
   elim : n. { left. by exists 0. }
@@ -351,23 +393,16 @@ Proof.
   - right. exists m. lia.
   - left. exists (S m). lia.
 Qed.
+*)
 
-(* induction principle wrt. a decreasing measure f *)
-(* example: elim /(measure_ind length) : l. *)
-Lemma measure_ind {X : Type} (f : X -> nat) (P : X -> Prop) :
-  (forall x, (forall y, f y < f x -> P y) -> P x) -> forall (x : X), P x.
-Proof.
-  exact: (well_founded_ind (Wf_nat.well_founded_lt_compat X f _ (fun _ _ => id)) P).
-Qed.
+
+
 
 Lemma HALF_spec X p q v offset :
   let x := vec_pos v X in let a := vec_pos v A in
   A <> X ->
   (offset, HALF X p q offset) // (offset, v) ->>
-    match half x with
-    | inl m => (p, vec_change (vec_change v X (a+m)) A 0)
-    | inr m => (q, vec_change (vec_change v X (a+m)) A 0)
-    end.
+    let '(m, b) := half x in (if b then p else q, vec_change (vec_change v X (a+m)) A 0).
 Proof.
   move=> /= HX. have H' : forall i, offset + i = i + offset by lia.
   apply: sss_compute_trans.
@@ -404,7 +439,580 @@ Proof.
   apply: Q_step_spec'. { done. }
   apply: IH. { rewrite !(vec_norm HX). lia. }
   rewrite !(vec_norm HX) /=.
-  have := half_spec n. case: (half n).
-  - move=> m ?. rewrite !(vec_norm HX). congr pair. congr vec_change. congr vec_change. lia.
-  - move=> m ?. rewrite !(vec_norm HX). congr pair. congr vec_change. congr vec_change. lia.
+  have := half_spec n. case: (half n) => m [] ->.
+  - rewrite !(vec_norm HX). congr pair. congr vec_change. congr vec_change. lia.
+  - rewrite !(vec_norm HX). congr pair. congr vec_change. congr vec_change. lia.
+Qed.
+
+(* IF X = 0 then GOTO p else GOTO q *)
+Definition BR (X: counter) (p q: nat) (offset: nat) : list mm_instr :=
+  let i := offset in [DEC X (JMP_length + 1 + i)] ++
+  let i := 1 + i in JMP p i ++
+  let i := JMP_length + i in [INC X] ++
+  let i := 1 + i in JMP q i.  
+
+Lemma BR_spec X p q v offset :
+  let x := vec_pos v X in
+  (offset, BR X p q offset) // (offset, v) ->> (if x is 0 then p else q, v).
+Proof.
+  move=> /=. have H' : forall i, offset + i = i + offset by lia.
+  case EX: (vec_pos v X) => [|n].
+  - apply: (Q_step_spec' _ _ 0). { by rewrite /= EX. }
+    apply: sss_compute_trans.
+    { apply: (subcode_sss_compute (P := (_, JMP _ _))).
+      { eexists _, _. done. }
+      rewrite ?H'. by apply: JMP_spec. }
+    by apply: sss_compute_refl'.
+  - apply: (Q_step_spec' _ _ 0). { by rewrite /= EX. }
+    apply: Q_step_spec'. { done. }
+    apply: sss_compute_trans.
+    { apply: (subcode_sss_compute (P := (_, JMP _ _))).
+      { eexists _, _. rewrite /BR. by do 2 rewrite [LHS]app_assoc. }
+      rewrite ?H'. by apply: JMP_spec. }
+    apply: sss_compute_refl'. congr pair.
+    by rewrite (vec_change_eq erefl) vec_change_idem -EX vec_change_same.
+Qed.
+
+Definition BR_length := length (BR A 0 0 0).
+Arguments BR_length : simpl never.
+
+Lemma half_spec_odd n : half ((n + n + 1) * 2 ^ 0) = (n, false).
+Proof.
+  have := half_spec ((n + n + 1) * 2 ^ 0).
+  case: (half _) => m [] /= *; congr pair; lia.
+Qed.
+
+Lemma half_spec_even n m : half ((n + n + 1) * 2 ^ (S m)) = ((n + n + 1) * 2 ^ m, true).
+Proof.
+  have := half_spec ((n + n + 1) * 2 ^ (S m)).
+  case: (half _) => k []; rewrite /= => ?; congr pair; lia.
+Qed.
+
+(* IF X = (n+n+1)*2^m THEN X := n AND Y := m *)
+Definition UNPACK (X Y: counter) (offset: nat) : list mm_instr :=
+  let i := offset in BR X 0 (BR_length + i) i ++
+  let i := BR_length + i in ZERO A i ++
+  let i := ZERO_length + i in ZERO Y i ++
+  let j := ZERO_length + i in HALF X (HALF_length + j) (JMP_length + 1 + HALF_length + j) j ++
+  let i := HALF_length + j in [INC Y] ++
+  let i := 1 + i in JMP j i.
+
+Definition UNPACK_length := length (UNPACK A A 0).
+
+Lemma UNPACK_spec {X Y m n v offset} :
+  let x := vec_pos v X in
+  x = (n + n + 1) * (2 ^ m) ->
+  A <> X -> A <> Y -> X <> Y ->
+  (offset, UNPACK X Y offset) // (offset, v) ->>
+    (UNPACK_length + offset, vec_change (vec_change (vec_change v X n) Y m) A 0).
+Proof.
+  move=> /= H'X HX HY HXY. have H' : forall i, offset + i = i + offset by lia.
+  apply: sss_compute_trans.
+  { apply: (subcode_sss_compute (P := (_, BR _ _ _ _))).
+    { by eexists [], _. }
+    rewrite ?H'. by apply: BR_spec. }
+  have ->: vec_pos v X = S (vec_pos v X - 1).
+  { rewrite H'X. have := Nat.pow_nonzero 2 m. lia. }
+  apply: sss_compute_trans.
+  { apply: (subcode_sss_compute (P := (_, ZERO _ _))).
+    { by eexists _, _. }
+    rewrite ?H'. by apply: ZERO_spec. }
+  apply: sss_compute_trans.
+  { apply: (subcode_sss_compute (P := (_, ZERO _ _))).
+    { eexists _, _. by rewrite /UNPACK [LHS]app_assoc. }
+    rewrite ?H'. by apply: ZERO_spec. }
+  suff : forall v' w', 
+    w' = vec_change (vec_change v' X n) Y (m + vec_pos v' Y) ->
+    vec_pos v' X = (n + n + 1) * 2 ^ m ->
+    vec_pos v' A = 0 ->
+    (offset, UNPACK X Y offset) //
+    (ZERO_length + BR_length + ZERO_length + offset, v') ->> (UNPACK_length + offset, w').
+  { apply.
+    - by rewrite !(vec_norm HXY) !(vec_norm HY) !(vec_norm HX) Nat.add_0_r.
+    - by rewrite !(vec_norm HXY) !(vec_norm HX).
+    - by rewrite !(vec_norm HY). }
+  elim: m {H'X}.
+  { move=> v' w' -> H'v' H''v'.
+    apply: sss_compute_trans.
+    { apply: (subcode_sss_compute (P := (_, HALF _ _ _ _))).
+      { eexists _, _. rewrite /UNPACK. by do 2 rewrite [LHS]app_assoc. }
+      rewrite ?H'. by apply: HALF_spec. }
+    rewrite H'v' half_spec_odd.
+    apply: sss_compute_refl'. congr pair.
+    rewrite H''v' !Nat.add_0_l !(vec_norm HXY) !(vec_norm (nesym HX)).
+    congr vec_change. by rewrite vec_change_same'. }
+  move=> m IH v' w' -> H'v' H''v'.
+  apply: sss_compute_trans.
+  { apply: (subcode_sss_compute (P := (_, HALF _ _ _ _))).
+    { eexists _, _. rewrite /UNPACK. by do 2 rewrite [LHS]app_assoc. }
+    rewrite ?H'. by apply: HALF_spec. }
+  rewrite H'v' half_spec_even.
+  rewrite !Nat.add_assoc. apply: Q_step_spec'. { done. }
+  apply: sss_compute_trans.
+  { apply: (subcode_sss_compute (P := (_, JMP _ _))).
+    { eexists _, _. rewrite /UNPACK. by do 4 rewrite [LHS]app_assoc. }
+    rewrite ?H'. by apply: JMP_spec. }
+  apply: IH.
+  - do ? rewrite ?(vec_norm (nesym HY)) ?(vec_norm (nesym HX)) ?(vec_norm HXY).
+    rewrite (vec_change_same' v' A 0 H''v').
+    congr vec_change. congr vec_change. lia.
+  - by rewrite !(vec_norm HXY) !(vec_norm HX) H''v'.
+  - by rewrite !(vec_norm HY).
+Qed.
+
+(*
+(* IF X = (n+n+1)*2^m THEN X := n AND Y := m *)
+Definition UNPACK (X Y: counter) (offset: nat) : list mm_instr :=
+  let i := offset in BR X 0 (BR_length + i) i ++
+  let i := BR_length + i in ZERO A i ++
+  let j := ZERO_length + i in HALF X (HALF_length + j) (JMP_length + 1 + HALF_length + j) j ++
+  let i := HALF_length + j in [INC Y] ++
+  let i := 1 + i in JMP j i.
+
+Definition UNPACK_length := length (UNPACK A A 0).
+
+Lemma UNPACK_spec X Y m n v offset :
+  let x := vec_pos v X in
+  let y := vec_pos v Y in
+  x = (n+n+1) * (2 ^ m) ->
+  A <> X -> A <> Y -> X <> Y ->
+  (offset, UNPACK X Y offset) // (offset, v) ->>
+    (UNPACK_length + offset, vec_change (vec_change (vec_change v X n) Y (m+y)) A 0).
+Proof.
+  move=> /= H'X HX HY HXY. have H' : forall i, offset + i = i + offset by lia.
+  apply: sss_compute_trans.
+  { apply: (subcode_sss_compute (P := (_, BR _ _ _ _))).
+    { by eexists [], _. }
+    rewrite ?H'. by apply: BR_spec. }
+  have ->: vec_pos v X = S (vec_pos v X - 1).
+  { rewrite H'X. have := Nat.pow_nonzero 2 m. lia. }
+  apply: sss_compute_trans.
+  { apply: (subcode_sss_compute (P := (_, ZERO _ _))).
+    { by eexists _, _. }
+    rewrite ?H'. by apply: ZERO_spec. }
+  move Ew: (w in _ // _ ->> (_, w)) => w.
+  elim: m v H'X w Ew.
+  { move=> v H'X ? <-.
+    apply: sss_compute_trans.
+    { apply: (subcode_sss_compute (P := (_, HALF _ _ _ _))).
+      { eexists _, _. by rewrite /UNPACK [LHS]app_assoc. }
+      rewrite ?H'. by apply: HALF_spec. }
+    rewrite !(vec_norm HX) H'X half_spec_odd.
+    apply: sss_compute_refl'. congr pair.
+    by rewrite !Nat.add_0_l !(vec_norm HX) !(vec_norm HXY). }
+  move=> m IH v H'X ? <-.
+  apply: sss_compute_trans.
+  { apply: (subcode_sss_compute (P := (_, HALF _ _ _ _))).
+    { eexists _, _. by rewrite /UNPACK [LHS]app_assoc. }
+    rewrite ?H'. by apply: HALF_spec. }
+  rewrite !(vec_norm HX) H'X half_spec_even.
+  rewrite !Nat.add_assoc. apply: Q_step_spec'. { done. }
+  apply: sss_compute_trans.
+  { apply: (subcode_sss_compute (P := (_, JMP _ _))).
+    { eexists _, _. rewrite /UNPACK. by do 3 rewrite [LHS]app_assoc. }
+    rewrite ?H'. by apply: JMP_spec. }
+  rewrite !(vec_norm HX) !(vec_norm HY).
+  apply: IH. { by rewrite !(vec_norm HXY). }
+  rewrite !(vec_norm HXY). congr vec_change. congr vec_change. congr vec_change. lia.
+Qed.
+*)
+
+Definition enc_pair (m n: nat) := (n+n+1)*(2^m).
+
+Import L (term, var, app, lam).
+
+Fixpoint enc_term (s: term) : nat :=
+  match s with
+  | var n => enc_pair 0 n
+  | lam s => enc_pair 1 (enc_term s)
+  | app s t => enc_pair (2 + enc_term t) (enc_term s)
+  end.
+
+Fixpoint enc_list (ns : list nat) : nat :=
+  match ns with
+  | [] => 0
+  | n::ns => enc_pair n (enc_list ns)
+  end.
+
+Fixpoint enc_closure (u: eterm) :=
+  match u with
+  | closure ctx s => enc_pair (enc_list (map enc_closure ctx)) (enc_term s)
+  end.
+
+Definition enc_cs ctx := enc_list (map enc_closure ctx).
+Arguments enc_cs !ctx /.
+
+Lemma HUA : A <> U.
+Proof. done. Qed.
+
+
+Lemma counters_eta (v : vec nat 5) :
+  v = Vector.hd v ## 
+    Vector.hd (VectorDef.tl v) ## 
+    Vector.hd (VectorDef.tl (VectorDef.tl v)) ## 
+    Vector.hd (VectorDef.tl (VectorDef.tl (VectorDef.tl v))) ##
+    Vector.hd (VectorDef.tl (VectorDef.tl (VectorDef.tl (VectorDef.tl v)))) ##
+    Vector.tl (VectorDef.tl (VectorDef.tl (VectorDef.tl (VectorDef.tl v)))).
+Proof.
+  by do 5 (rewrite [LHS](Vector.eta v); congr Vector.cons; move: (Vector.tl v) => {}v).
+Qed.
+
+Definition CASE_VAR0 (p: nat) (offset : nat) : list mm_instr :=
+  let i := offset in UNPACK CTX U i ++
+  let i := UNPACK_length + i in UNPACK U CTX i ++
+  let i := UNPACK_length + i in JMP p i.
+
+Definition CASE_VAR0_length := length (CASE_VAR0 0 0).
+
+Lemma CASE_VAR0_spec ctx' t' ctx p v offset :
+  vec_pos v CTX = enc_cs ((closure ctx' t') :: ctx) ->
+  (offset, CASE_VAR0 p offset) // (offset, v) ->>
+    (p, vec_change (vec_change (vec_change v U (enc_term t')) CTX (enc_cs ctx')) A 0).
+Proof.
+  move=> /= Hv. have H' : forall i, offset + i = i + offset by lia.
+  apply: sss_compute_trans.
+  { apply: (subcode_sss_compute (P := (_, UNPACK _ _ _))).
+    { by eexists [], _. }
+    rewrite ?H'. by apply: (UNPACK_spec Hv). }
+  move Ev': (vec_change _ A 0) => v'.
+  apply: sss_compute_trans.
+  { apply: (subcode_sss_compute (P := (_, UNPACK _ _ _))).
+    { by eexists _, _. }
+    rewrite ?H'.
+    have /= /UNPACK_spec : vec_pos v' U = enc_closure (closure ctx' t').
+    { by rewrite -Ev' (counters_eta v). } by apply. }
+  apply: sss_compute_trans.
+  { apply: (subcode_sss_compute (P := (_, JMP _ _))).
+    { eexists _, _. by rewrite /CASE_VAR0 [LHS]app_assoc. }
+    rewrite ?H'. by apply: JMP_spec. }
+  apply: sss_compute_refl'. congr pair.
+  by rewrite -Ev' (counters_eta v).
+Qed.
+
+Definition CASE_VARS (p: nat) (offset : nat) : list mm_instr :=
+  let i := offset in UNPACK CTX B i ++
+  let i := UNPACK_length + i in ZERO B i ++
+  let i := ZERO_length + i in PACK U B i ++
+  let i := PACK_length + i in JMP p i.
+
+Definition CASE_VARS_length := length (CASE_VARS 0 0).
+
+Lemma CASE_VARS_spec u ctx n p v offset :
+  vec_pos v CTX = enc_cs (u :: ctx) ->
+  vec_pos v U = n ->
+  vec_pos v B = 0 ->
+  (offset, CASE_VARS p offset) // (offset, v) ->>
+    (p, vec_change (vec_change (vec_change v U (enc_term (var n))) CTX (enc_cs ctx)) A 0).
+Proof.
+  move=> /= HCTX HU HB. have H' : forall i, offset + i = i + offset by lia.
+  apply: sss_compute_trans.
+  { apply: (subcode_sss_compute (P := (_, UNPACK _ _ _))).
+    { by eexists [], _. }
+    rewrite ?H'. by apply: (UNPACK_spec HCTX). }
+  apply: sss_compute_trans.
+  { apply: (subcode_sss_compute (P := (_, ZERO _ _))).
+    { by eexists _, _. }
+    rewrite ?H'. by apply: ZERO_spec. }
+  apply: sss_compute_trans.
+  { apply: (subcode_sss_compute (P := (_, PACK _ _ _))).
+    { eexists _, _. by rewrite /CASE_VARS [LHS]app_assoc. }
+    rewrite ?H'. by apply: PACK_spec. }
+  apply: sss_compute_trans.
+  { apply: (subcode_sss_compute (P := (_, JMP _ _))).
+    { eexists _, _. rewrite /CASE_VARS. by do 2 rewrite [LHS]app_assoc. }
+    rewrite ?H'. by apply: JMP_spec. }
+  apply: sss_compute_refl'. move: HCTX HU HB. rewrite (counters_eta v) /=.
+  by move=> ? -> ->.
+Qed.
+
+Definition CASE_APP (p: nat) (offset : nat) : list mm_instr :=
+  let i := offset in PACK B CTX i ++
+  let i := PACK_length + i in PACK TS B i ++
+  let i := PACK_length + i in COPY TS CTX i ++
+  let i := COPY_length + i in UNPACK CTX B i ++
+  let i := UNPACK_length + i in UNPACK B CTX i ++
+  let i := UNPACK_length + i in JMP p i ++
+  [].
+
+Definition CASE_APP_length := length (CASE_APP 0 0).
+
+Arguments Nat.pow : simpl never.
+
+Lemma CASE_APP_spec ts ctx t p v offset :
+  vec_pos v TS = enc_cs ts ->
+  vec_pos v CTX = enc_cs ctx ->
+  vec_pos v B = enc_term t ->
+  (offset, CASE_APP p offset) // (offset, v) ->>
+    (p, vec_change (vec_change v TS (enc_cs ((closure ctx t)::ts))) A 0).
+Proof.
+  move=> /= HTS HCTX HB. have H' : forall i, offset + i = i + offset by lia.
+  apply: sss_compute_trans.
+  { apply: (subcode_sss_compute (P := (_, PACK _ _ _))).
+    { by eexists [], _. }
+    rewrite ?H'. by apply: PACK_spec. }
+  apply: sss_compute_trans.
+  { apply: (subcode_sss_compute (P := (_, PACK _ _ _))).
+    { by eexists _, _. }
+    rewrite ?H'. by apply: PACK_spec. }
+  apply: sss_compute_trans.
+  { apply: (subcode_sss_compute (P := (_, COPY _ _ _))).
+    { eexists _, _. rewrite /CASE_APP. by do 1 rewrite [LHS]app_assoc. }
+    rewrite ?H'. by apply: COPY_spec. }
+  do ? (rewrite ?(vec_change_eq erefl); try (rewrite vec_change_neq; first done)).
+  apply: sss_compute_trans.
+  { apply: (subcode_sss_compute (P := (_, UNPACK _ _ _))).
+    { eexists _, _. rewrite /CASE_APP. by do 2 rewrite [LHS]app_assoc. }
+    rewrite ?H'. apply: UNPACK_spec; [|done ..].
+    do ? (rewrite ?(vec_change_eq erefl); try (rewrite vec_change_neq; first done)).
+    by rewrite Nat.add_0_r. }
+  apply: sss_compute_trans.
+  { apply: (subcode_sss_compute (P := (_, UNPACK _ _ _))).
+    { eexists _, _. rewrite /CASE_APP. by do 3 rewrite [LHS]app_assoc. }
+    rewrite ?H'. apply: UNPACK_spec; [|done ..].
+    do ? (rewrite ?(vec_change_eq erefl); try (rewrite vec_change_neq; first done)).
+    done. }
+  apply: sss_compute_trans.
+  { apply: (subcode_sss_compute (P := (_, JMP _ _))).
+    { eexists _, _. rewrite /CASE_APP. by do 4 rewrite [LHS]app_assoc. }
+    rewrite ?H'. by apply: JMP_spec. }
+  apply: sss_compute_refl'. move: HTS HCTX HB. rewrite (counters_eta v) /=.
+  by move=> -> -> ->.
+Qed.
+
+Definition CASE_LAM (p: nat) (offset : nat) : list mm_instr :=
+  let i := offset in UNPACK TS B i ++
+  let i := UNPACK_length + i in PACK CTX B i ++
+  let i := PACK_length + i in JMP p i ++
+  [].
+
+Definition CASE_LAM_length := length (CASE_LAM 0 0).
+
+Lemma CASE_LAM_spec t ts ctx p v offset :
+  vec_pos v TS = enc_cs (t :: ts) ->
+  vec_pos v CTX = enc_cs ctx ->
+  vec_pos v B = 0 ->
+  (offset, CASE_LAM p offset) // (offset, v) ->>
+    (p, vec_change (vec_change (vec_change v TS (enc_cs ts)) CTX (enc_cs (t::ctx))) A 0).
+Proof.
+  move=> /= HTS HCTX HB. have H' : forall i, offset + i = i + offset by lia.
+  apply: sss_compute_trans.
+  { apply: (subcode_sss_compute (P := (_, UNPACK _ _ _))).
+    { by eexists [], _. }
+    rewrite ?H'. by apply: (UNPACK_spec HTS). }
+  apply: sss_compute_trans.
+  { apply: (subcode_sss_compute (P := (_, PACK _ _ _))).
+    { by eexists _, _. }
+    rewrite ?H'. by apply: PACK_spec. }
+  apply: sss_compute_trans.
+  { apply: (subcode_sss_compute (P := (_, JMP _ _))).
+    { eexists _, _. rewrite /CASE_VARS. by do 1 rewrite [LHS]app_assoc. }
+    rewrite ?H'. by apply: JMP_spec. }
+  apply: sss_compute_refl'. move: HTS HCTX HB. rewrite (counters_eta v) /=.
+  by move=> ? -> ->.
+Qed.
+
+Definition NOOP (offset : nat) : list mm_instr :=
+  JMP (JMP_length + offset) offset.
+
+Definition NOOP_length := length (NOOP 0).
+
+Lemma NOOP_spec v offset :
+  (offset, NOOP offset) // (offset, v) -+> (NOOP_length+offset, v).
+Proof.
+  exists 2. split; first by lia.
+  apply: in_sss_steps_S. { by apply: (Q_step_spec _ offset 0). }
+  apply: in_sss_steps_S. { apply: Q_step_spec. by rewrite /= (vec_change_eq erefl). }
+  rewrite vec_change_idem vec_change_same.
+  by apply: in_sss_steps_0.
+Qed.
+
+Definition PROG (offset : nat) : list mm_instr :=
+  let i := offset in NOOP i ++
+  let i := NOOP_length + i in UNPACK U B i ++
+  let i := UNPACK_length + i in [DEC B (CASE_VARS_length+CASE_VAR0_length+2+i)] ++
+  (* var _ CASE *) let i := 1 + i in [DEC U (CASE_VAR0_length+1+i)] ++
+  (* var 0 CASE *) let i := 1 + i in CASE_VAR0 offset i ++
+  (* var (S n) CASE *) let i := CASE_VAR0_length + i in CASE_VARS offset i ++
+  let i := CASE_VARS_length + i in [DEC B (CASE_LAM_length+1+i)] ++
+  (* lam s CASE *) let i := 1 + i in CASE_LAM offset i ++
+  (* app s t CASE *) let i := CASE_LAM_length + i in CASE_APP offset i ++
+  [].
+
+Definition Krivine_step : (list eterm * list eterm * term) -> option (list eterm * list eterm * term) :=
+  fun '(ts, ctx, t) =>
+  match t with
+  | var 0 => 
+      match ctx with
+      | [] => None
+      | (closure ctx t)::_ => Some (ts, ctx, t)
+      end
+  | var (S n) =>
+      match ctx with
+      | [] => None
+      | _::ctx => Some (ts, ctx, var n)
+      end
+  | lam s =>
+      match ts with
+      | [] => None
+      | t::ts => Some (ts, t::ctx, s)
+      end
+  | app s t => Some ((closure ctx t)::ts, ctx, s)
+  end.
+
+Lemma iter_plus {X} {f : X -> X} {x : X} n m : Nat.iter (n + m) f x = Nat.iter m f (Nat.iter n f x).
+Proof.
+  elim: m; first by rewrite Nat.add_0_r.
+  move=> m /= <-. by have ->: n + S m = S n + m by lia.
+Qed.
+
+Lemma oiter_None {X : Type} (f : X -> option X) k : Nat.iter k (obind f) None = None.
+Proof. elim: k; [done | by move=> /= ? ->]. Qed.
+
+Lemma Krivine_step_spec ts ctx t : halt_cbn ts ctx t <-> 
+  exists k ctx' t', Nat.iter k (obind Krivine_step) (Some (ts, ctx, t)) = Some ([], ctx', lam t').
+Proof.
+  split.
+  - elim.
+    1-4: by move=> > ? [n] [ctx'] [t'] IH; exists (S n), ctx', t'; rewrite (iter_plus 1 n).
+    move=> >. exists 0. by do 2 eexists.
+  - move=> [k] [ctx'] [t'].
+    elim: k ts ctx t. { move=> > [-> -> ->]. by apply: halt_lam. }
+    move=> k IH ts ctx t. rewrite (iter_plus 1 k) /=.
+    case: t.
+    + move=> [|n].
+      * case: ctx; first by rewrite oiter_None.
+        move=> [? ?] ? /IH ?. by apply: halt_var_0.
+      * case: ctx; first by rewrite oiter_None.
+        move=> [? ?] ? /IH ?. by apply: halt_var_S.
+    + move=> ?? /IH ?. by apply: halt_app.
+    + move=> ?. case: ts; first by rewrite oiter_None.
+      move=> ?? /IH ?. by apply: halt_lam_ts.
+Qed.
+
+Lemma HAB : A <> B.
+Proof. done. Qed.
+
+Lemma HACTX : A <> CTX.
+Proof. done. Qed.
+
+Lemma HBCTX : B <> CTX.
+Proof. done. Qed.
+
+Lemma HCTXU : CTX <> U.
+Proof. done. Qed.
+
+Lemma HAU : A <> U.
+Proof. done. Qed.
+
+Lemma HBU : B <> U.
+Proof. done. Qed.
+
+Lemma PROG_spec ts ctx t v ts' ctx' t' offset :
+  vec_pos v TS = enc_cs ts ->
+  vec_pos v CTX = enc_cs ctx ->
+  vec_pos v U = enc_term t ->
+  Krivine_step (ts, ctx, t) = Some (ts', ctx', t') ->
+  exists w, 
+    vec_pos w TS = enc_cs ts' /\
+    vec_pos w CTX = enc_cs ctx' /\
+    vec_pos w U = enc_term t' /\
+    (offset, PROG offset) // (offset, v) -+> (offset, w).
+Proof.
+  have H' : forall i, offset + i = i + offset by lia.
+  case: t.
+  - move=> [|n] /=; (case: ctx; first done).
+    + (* case (var 0) *)
+      move=> [ctx'' t'' ?] H1v H2v H3v  [<- <- <-].
+      exists (vec_change (vec_change (vec_change (vec_change v U (enc_term t'')) CTX (enc_cs ctx'')) B 0) A 0).
+      split. { move: H1v. by rewrite (counters_eta v). }
+      split. { move: H2v. by rewrite (counters_eta v). }
+      split. { move: H3v. by rewrite (counters_eta v). }
+      apply: sss_progress_compute_trans.
+      { apply: (subcode_sss_progress (P := (_, NOOP _))).
+        { by eexists [], _. }
+        rewrite ?H'. by apply: NOOP_spec. }
+      apply: sss_compute_trans.
+      { apply: (subcode_sss_compute (P := (_, UNPACK _ _ _))).
+        { by eexists _, _. }
+        rewrite ?H'. by apply: (UNPACK_spec H3v). }
+      rewrite ?Nat.add_assoc. apply: Q_step_spec'. { by rewrite /= !(vec_norm HAB). }
+      rewrite ?Nat.add_assoc. apply: Q_step_spec'. { by rewrite /= !(vec_norm HAU) !(vec_norm HBU). }
+      apply: sss_compute_trans.
+      { apply: (subcode_sss_compute (P := (_, CASE_VAR0 _ _))).
+        { eexists _, _. rewrite /PROG. by do 3 rewrite [LHS]app_assoc. }
+        rewrite ?H'. apply: CASE_VAR0_spec.
+        do ? (rewrite vec_change_neq; first done). by eassumption. }
+      apply: sss_compute_refl'. by rewrite (counters_eta v).
+    + (* case (var (S n)) *)
+      move=> ? ctx'' H1v H2v H3v  [<- <- <-].
+      exists (vec_change (vec_change (vec_change (vec_change v U (enc_term (var n))) CTX (enc_cs ctx'')) B 0) A 0).
+      split. { move: H1v. by rewrite (counters_eta v). }
+      split. { move: H2v. by rewrite (counters_eta v). }
+      split. { move: H3v. by rewrite (counters_eta v). }
+      apply: sss_progress_compute_trans.
+      { apply: (subcode_sss_progress (P := (_, NOOP _))).
+        { by eexists [], _. }
+        rewrite ?H'. by apply: NOOP_spec. }
+      apply: sss_compute_trans.
+      { apply: (subcode_sss_compute (P := (_, UNPACK _ _ _))).
+        { by eexists _, _. }
+        rewrite ?H'. by apply: (UNPACK_spec H3v). }
+      rewrite ?Nat.add_assoc. apply: Q_step_spec'. { by rewrite /= !(vec_norm HAB). }
+      rewrite ?Nat.add_assoc. apply: Q_step_spec'. { by rewrite /= !(vec_norm HAU) !(vec_norm HBU). }
+      apply: sss_compute_trans.
+      { apply: (subcode_sss_compute (P := (_, CASE_VARS _ _))).
+        { eexists _, _. rewrite /PROG. by do 4 rewrite [LHS]app_assoc. }
+        rewrite ?H'. apply: CASE_VARS_spec.
+        - do ? (rewrite vec_change_neq; first done). by eassumption.
+        - by rewrite (vec_change_eq erefl).
+        - do ? (rewrite vec_change_neq; first done). by rewrite (vec_change_eq erefl). }
+      apply: sss_compute_refl'. by rewrite (counters_eta v).
+  - (* case (app s t) *)
+    move=> s t H1v H2v H3v [<- <- <-].
+    exists (vec_change (vec_change (vec_change (vec_change v U (enc_term s)) B (enc_term t)) TS (enc_cs ((closure ctx t)::ts))) A 0).
+    split. { move: H1v. by rewrite (counters_eta v). }
+    split. { move: H2v. by rewrite (counters_eta v). }
+    split. { move: H3v. by rewrite (counters_eta v). }
+    apply: sss_progress_compute_trans.
+    { apply: (subcode_sss_progress (P := (_, NOOP _))).
+      { by eexists [], _. }
+      rewrite ?H'. by apply: NOOP_spec. }
+    apply: sss_compute_trans.
+    { apply: (subcode_sss_compute (P := (_, UNPACK _ _ _))).
+      { by eexists _, _. }
+      rewrite ?H'. by apply: (UNPACK_spec H3v). }
+    rewrite ?Nat.add_assoc. apply: Q_step_spec'. { by rewrite /= -/enc_term !(vec_norm HAB). }
+    rewrite ?Nat.add_assoc. apply: Q_step_spec'. { by rewrite /= !(vec_norm HAB). }
+    apply: sss_compute_trans.
+    { apply: (subcode_sss_compute (P := (_, CASE_APP _ _))).
+      { eexists _, _. rewrite /PROG. by do 7 rewrite [LHS]app_assoc. }
+      rewrite ?H'. apply: CASE_APP_spec.
+      - do ? (rewrite vec_change_neq; first done). by eassumption.
+      - do ? (rewrite vec_change_neq; first done). by eassumption.
+      - do ? (rewrite vec_change_neq; first done). by rewrite (vec_change_eq erefl). }
+    apply: sss_compute_refl'. by rewrite (counters_eta v).
+  - move=> s. case: ts; first done.
+    move=> t'' ts'' H1v H2v H3v [<- <- <-].
+    exists (vec_change (vec_change (vec_change (vec_change (vec_change v U (enc_term s)) TS (enc_cs ts'')) CTX (enc_cs (t''::ctx))) B 0) A 0).
+    split. { move: H1v. by rewrite (counters_eta v). }
+    split. { move: H2v. by rewrite (counters_eta v). }
+    split. { move: H3v. by rewrite (counters_eta v). }
+    apply: sss_progress_compute_trans.
+    { apply: (subcode_sss_progress (P := (_, NOOP _))).
+      { by eexists [], _. }
+      rewrite ?H'. by apply: NOOP_spec. }
+    apply: sss_compute_trans.
+    { apply: (subcode_sss_compute (P := (_, UNPACK _ _ _))).
+      { by eexists _, _. }
+      rewrite ?H'. by apply: (UNPACK_spec H3v). }
+    rewrite ?Nat.add_assoc. apply: Q_step_spec'. { by rewrite /= -/enc_term !(vec_norm HAB). }
+    rewrite ?Nat.add_assoc. apply: Q_step_spec'. { by rewrite /= !(vec_norm HAB). }
+    apply: sss_compute_trans.
+    { apply: (subcode_sss_compute (P := (_, CASE_LAM _ _))).
+      { eexists _, _. rewrite /PROG. by do 6 rewrite [LHS]app_assoc. }
+      rewrite ?H'. apply: CASE_LAM_spec.
+      - do ? (rewrite vec_change_neq; first done). by eassumption.
+      - do ? (rewrite vec_change_neq; first done). by eassumption.
+      - do ? (rewrite vec_change_neq; first done). by rewrite (vec_change_eq erefl). }
+    apply: sss_compute_refl'. by rewrite (counters_eta v).
 Qed.
